Mem.v
@@ -1,0 +1,32 @@
+From Coq Require Import Lists.List.
+
+Definition mem (A : Type) := list (nat * A). 
+
+Fixpoint get {A : Type} (m : mem A) i default :=
+  match m with
+  | nil => default
+  | (i', a') :: m' => if Nat.eqb i i' then a' else get m' i default 
+  end.
+
+Definition set {A : Type} (m : mem A) i a :=
+  (i, a) :: m.
+
+Definition length {A : Type} (m : mem A) :=
+  fold_left (fun x y => max x (fst y)) m 0. 
+
+(* Proofs *)
+
+Lemma get_set_eq : forall {A} default (m : mem A) i a,
+  get ((i, a) :: m) i default = a.
+Proof.
+  intros. simpl. rewrite PeanoNat.Nat.eqb_refl. reflexivity.
+Qed.
+
+Lemma get_set_neq : forall {A} (m : mem A) i i' a,
+  i <> i' ->
+  get ((i', a) :: m) i = get m i.
+Proof.
+  intros * Hneq. eapply PeanoNat.Nat.eqb_neq in Hneq.
+  simpl. rewrite Hneq. reflexivity.
+Qed.
+
